tests/Binder_Datatype_Tests.thy
@@ -7,5 +7,8 @@ binder_datatype ('a, 'b, free 'c, 'd, 'f, bound 'e) T1 =
 | Bdr1 x::'a t::"('a, 'b, 'c, 'd, 'f, 'e) T1" binds x in t
 | Bdr2 x::'b "(t::('a, 'b, 'c, 'd, 'f, 'e) T1) list" binds x in t
 | Passive 'c 'd 'e 'f
+for rel: match_T1
+
+term "match_T1"
 
 end
